src/PlutusIR/Semantics/Static/normaliser_STLC/alpha/alpha.v
@@ -16,46 +16,6 @@ Unset Strict Implicit.
 Unset Printing Implicit Defensive.
 From PlutusCert Require Import STLC_named ARS util.
 
-(** **** Capms lemmas *)
-Lemma capms_var sigma X t:
-  lookup X sigma = Some t -> capms sigma (tmvar X) = t.
-Proof. 
-  rewrite capms_equation_1. 
-  by move ->.
-Qed.
-
-Lemma capms_lam X B sigma s :
-  capms sigma (tmlam X B s) = 
-    tmlam (fresh2 ((X, tmvar X)::sigma) s) B (capms sigma (rename X (fresh2 ((X, tmvar X)::sigma) s) s)).
-Proof.
-  rewrite capms_equation_2.
-  reflexivity.
-Qed.
-
-(** **** One-Step Reduction *)
-
-(* Set Implicit Arguments.
-Unset Strict Implicit.
-Unset Printing Implicit Defensive.
-
-Delimit Scope prop_scope with PROP.
-Open Scope prop_scope. *)
-
-(* Alpha reduction based on Andrej Bauer (Computer Science stack exchange)*)
-(* Inductive relation for:
-
-equalVar :: [(Var,Var)] -> Var -> Var -> Bool
-equalVar [] x y = (x == y)
-equalVar ((x,y):bound) z w = (x == z && y == w) || (x /= z && y /= w && equalVar bound z w)
-
-equal' :: [(Var, Var)] -> Term -> Term -> Bool
-equal' bound (Belong x1 y1) (Belong x2 y2) = (equalVar bound x1 x2 && equalVar bound y1 y2)
-equal' bound Bot Bot = True
-equal' bound (Imply u1 v1) (Imply u2 v2) = equal' bound u1 u2 && equal' bound v1 v2
-equal' bound (Forall x u) (Forall y v) = equal' ((x,y):bound) u v
-equal' _ _ _ = False
-
-*)
 Inductive AlphaVar : list (string * string) -> string -> string -> Set :=
 | alpha_var_refl x : AlphaVar [] x x
 | alpha_var_cons z w sigma :
@@ -70,31 +30,15 @@ Inductive Alpha : list (string * string) -> term -> term -> Set :=
 | alpha_var x y sigma : 
     AlphaVar sigma x y -> 
     Alpha sigma (tmvar x) (tmvar y)
-| alpha_lam x y A s1 s2 sigma :
+| alpha_lam B x y A s1 s2 sigma :
     Alpha ((x, y) :: sigma) s1 s2 -> 
-    Alpha sigma (tmlam x A s1) (tmlam y A s2)
-| alpha_app s1 s2 t1 t2 sigma :
+    Alpha sigma (@tmlam B x A s1) (@tmlam B y A s2)
+| alpha_app B s1 s2 t1 t2 sigma :
     Alpha sigma s1 s2 -> 
     Alpha sigma t1 t2 -> 
-    Alpha sigma (tmapp s1 t1) (tmapp s2 t2).
-
-Fixpoint swap (x y : string) (s : term) := 
-  match s with
-  | tmvar z => if z =? x then tmvar y else if z =? y then tmvar x else tmvar z
-  | tmlam z A s' => if z =? x then tmlam y A (swap x y s') else if z =? y then tmlam x A (swap x y s') else tmlam z A (swap x y s')
-  | tmapp s1 s2 => tmapp (swap x y s1) (swap x y s2)
-  end.
-
-Inductive AlphaSwap : term -> term -> Set :=
-| alphaswap_var x :
-  AlphaSwap (tmvar x) (tmvar x)
-| alphaswap_lam x y A s1 s2 :
-  AlphaSwap s1 (swap x y s2) -> 
-  AlphaSwap (tmlam x A s1) (tmlam y A s2)
-| alphaswap_app s1 s2 t1 t2 :
-  AlphaSwap s1 s2 -> 
-  AlphaSwap t1 t2 -> 
-  AlphaSwap (tmapp s1 t1) (tmapp s2 t2).
+    Alpha sigma (@tmapp B s1 t1) (@tmapp B s2 t2)
+| alpha_builtin R d :
+    Alpha R (tmbuiltin d) (tmbuiltin d).
 
 (* **** Properties of Alpha *)
 
@@ -115,86 +59,6 @@ Notation "sigma '⊢' t1 '~' t2" := (Alpha sigma t1 t2) (at level 40).
 
 (* Example of alpha equivalence *)
 
-
-(* TODO: Should we add the assumption that we are always substing in fresh stuff? *)
-(* TODO: Fresh with respect to what? *)
-Fixpoint rename2 (X Y : string) (T : term) : term :=
-  match T with
-  | tmvar X' => if X =? X' then tmvar Y else tmvar X'
-  | tmlam X' K1 T_body => if X =? X' then tmlam X' K1 T_body else tmlam X' K1 (rename2 X Y T_body)
-  | tmapp T1 T2 => tmapp (rename2 X Y T1) (rename2 X Y T2)
-end.
-
-(* Suppose s1 = x, and s2 = y. Then we have Alpha2 (renameTCA x y s1) s2
-    so yes.
-
-    What if s1 = y and s2 = y, then we have Alpha2 (renameTCA x y s1) s2 = Alpha2 y y = True
-    But we should not have Alpha2 (tmlam x A y) (tmlam y A y)... so no
-*)
-Inductive Alpha2 : term -> term -> Set:=
-| alpha2_var x :
-  Alpha2 (tmvar x) (tmvar x)
-| alpha2_app s1 s2 t1 t2 :
-  Alpha2 s1 s2 -> 
-  Alpha2 t1 t2 -> 
-  Alpha2 (tmapp s1 t1) (tmapp s2 t2)
-| alpha2_lam x y A s1 s2 :
-  Alpha2 (rename2 x y s1) (rename2 y x s2) ->  
-  Alpha2 (tmlam x A s1) (tmlam y A s2).
-
-Require Import Ascii.
-
-Inductive Fresh3 : string -> string -> string -> term -> term -> Set :=
-| fresh_var fr x y s1 s2 :
-    fr <> x -> 
-    fr <> y -> 
-    ~ In fr (tv s1) ->
-    ~ In fr (tv s2) ->
-    Fresh3 fr x y s1 s2.
-
-Definition fresh3 (x y : string) (s1 s2 : term) : string :=
-  "a" (* new*)
-  ++ String.concat EmptyString (
-    x :: y :: tv s1 ++ tv s2
-  ).
-
-Lemma fresh3_sound_complete :
-  forall x y s1 s2, Fresh3 (fresh3 x y s1 s2) x y s1 s2.
-Admitted.
-
-(* This is definition 3.1 in https://pdf.sciencedirectassets.com/271538/1-s2.0-S0304397512X00161/1-s2.0-S0304397512000667/main.pdf?X-Amz-Security-Token=IQoJb3JpZ2luX2VjEMH%2F%2F%2F%2F%2F%2F%2F%2F%2F%2FwEaCXVzLWVhc3QtMSJGMEQCIG%2BQqldD%2FjA7NoiWQ8LNNSiVisTNC0Bg6XND41y0KfGFAiAFFmELjxK%2FE%2FcIVfE3L9st4Og6PAdKhLiZyyBDiT8LECq8BQi6%2F%2F%2F%2F%2F%2F%2F%2F%2F%2F8BEAUaDDA1OTAwMzU0Njg2NSIMNeW5gtEinHpeKgTWKpAFBTCfszS77ANhiG%2Fcb%2FsSUt1skJsS%2FXVCRS0jhmCVGks3Yjl622BzjOcdpQYlTVUT2ohNGrxknOvHgVO4%2BcePabv3%2BfAiBGP8s1FOo5%2BH7pBpIhZ7eTKH%2FtvbEP%2BYNUh53QX%2F1wZQQH0oebBlfpTgKtZzii7b2oZI4ibLAOiUfc87x6lDARXz2ROdVZWq6F72kWkcU0cZflFE6hNRcXYiKlcKocu2EvAordoc0XfBhNkOQp%2Fgv%2FtuJeEr130nNMSWdzbRM2AaQ6UQGD8igj5rJJ8z%2FEWIFXQREwtYdiiXi1bJDly5cT7lzyOExLAay8dYV6LPBRRehx5XgaCVqz61z9VPrrWqs1A2zheM22Ryw6ertBj58pIa98jTNbD4STlG1akJV%2BFs2NBr3SDuiDxqEn%2F1FKZz5aOTFfPYjWtppYEZVsjEMtC19mQm8fFIyavO975zFRkJ0IEBWb05i680iC0iOKlhT%2BHLAlDoBmo%2BUje9HHSY5ICQ8LA8avTqPKZOrP%2B4N0CZqscyY0C%2BxSgmD7%2BhVEMFr4EGJv1lWFehonJPheA3Cgd75q4wvAHWa1dUwyXWdnNTr2PVloxTMVTdQswq84QnjDiQe%2FJYu6%2BjrYNSj8vKjfdtUiYbsD2PENBt31gooeo6Jb%2Bf82mh4xHDV6JZ07mTHYwJAkN%2FcjyGFOCRcYYDO4VjftIwnBv1%2BtlaD94BO%2Bxh2HJDbfXWh0ylRRCK9LraPDHTf6ZxnOj0kYsqKyWGO5CID3oyurbhFUowlkaRfyIrxgt%2F89pzVrQtFPryy3dR%2FJbcN4ynvS2hOh2fevptFHV2%2BiD2vM9KRFMbLsz4QgeeO2XzXgwcjXR9KX5UOxg6uu%2FqdtUA%2BCOFrH4wn8S9vAY6sgFY5l2eE1BY7RYQmFsouQcQRDqbBwHdTHBToqQ6Euo6wOOOQdZY5erdrUBAls%2BP5KnQZIDqAVNjbZ34e14BtHVzzDytH6mo3q%2Bg4gUWM5ON0qZy%2BqFuWQKzfnTu7TQisgjYR0OvxABy2D%2FkMSNZ71FEl7EyaWJLuol3EcTd8lyj5G4kBAv487tPpYEZHXczLT3JXPPEgWc96mNnp%2FyUFiQG8F3yy1UpPc5H3d%2BhF%2Bjj%2FlEb&X-Amz-Algorithm=AWS4-HMAC-SHA256&X-Amz-Date=20250121T094752Z&X-Amz-SignedHeaders=host&X-Amz-Expires=300&X-Amz-Credential=ASIAQ3PHCVTYVUNMHNK4%2F20250121%2Fus-east-1%2Fs3%2Faws4_request&X-Amz-Signature=398b562e375d1a16c7f60ab80429dfaf310a35e377e630760503b684f84da28c&hash=3dcb22b98618eeaa6529ad48b4a7b543abf03bc96650448909e29c5712e27c4b&host=68042c943591013ac2b2430a89b270f6af2c76d8dfd086a07176afe7c76c2c61&pii=S0304397512000667&tid=spdf-e832ba5a-7b88-43ab-846d-05556869c86e&sid=48b03c4275472545d69b5e31e4a1d3f9ea1agxrqb&type=client&tsoh=d3d3LnNjaWVuY2VkaXJlY3QuY29t&ua=080b5a51535050500f57&rr=905662a1e825d0b9&cc=nl
-Alpha equivalence equalities
-Roy L. Crole ∗
-
-We do not swap, but we are working with a fresh variable, so that cannot occur, so then we do not have to swap?
-*)
-Inductive Alpha3 : term -> term -> Set:=
-| alpha3_var x :
-  Alpha3 (tmvar x) (tmvar x)
-| alpha3_app s1 s2 t1 t2 :
-  Alpha3 s1 s2 -> 
-  Alpha3 t1 t2 -> 
-  Alpha3 (tmapp s1 t1) (tmapp s2 t2)
-| alpha3_lam x y A s1 s2 fr :
-  Fresh3 fr x y s1 s2 ->
-  Alpha3 (rename2 x fr s1) (rename2 y fr s2) ->  
-  Alpha3 (tmlam x A s1) (tmlam y A s2).
-
-
-Inductive Alpha4 : term -> term -> Set:=
-| alpha4_var x :
-  Alpha4 (tmvar x) (tmvar x)
-| alpha4_app s1 s2 t1 t2 :
-  Alpha4 s1 s2 -> 
-  Alpha4 t1 t2 -> 
-  Alpha4 (tmapp s1 t1) (tmapp s2 t2)
-| alpha4_lam x A s1 s2 :
-  Alpha4 s1 s2 ->
-  Alpha4 (tmlam x A s1) (tmlam x A s2)
-| alpha4_ren x y A s1 s1' :
-  s1' = rename2 x y s1 ->
-  Alpha4 (tmlam x A s1) (tmlam y A s1').
-
 (* **** Examples *)
 
 (* Example of alpha equivalence *)
@@ -202,7 +66,7 @@ Inductive Alpha4 : term -> term -> Set:=
 
 Lemma alpha_exampl x y y' A :
   x <> y -> y <> y' -> x <> y' -> 
-  Alpha [] (tmlam x A (tmlam y A (tmapp (tmvar x) (tmvar y)))) (tmlam y A (tmlam y' A (tmapp (tmvar y) (tmvar y')))).
+  Alpha [] (@tmlam Lam x A (@tmlam Lam y A (@tmapp App (tmvar x) (tmvar y)))) (@tmlam Lam y A (@tmlam Lam y' A (@tmapp App (tmvar y) (tmvar y')))).
 Proof.
   intros Hxy Hyy' Hxy'.
   apply alpha_lam.
@@ -213,104 +77,21 @@ Proof.
   - apply alpha_var. apply alpha_var_cons; reflexivity.
 Qed.
 
-Lemma alpha3_example x y A :
-  x <> y ->
-  Alpha3 (tmlam x A (tmvar x)) (tmlam y A (tmvar y)).
-Proof.
-  intros.
-  eapply alpha3_lam with (fr := fresh3 x y (tmvar x) (tmvar y)); auto.
-  - apply fresh3_sound_complete.
-  -
-  simpl.
-  repeat rewrite String.eqb_refl.
-  constructor.
-Qed.
-
-Lemma alpha3_example2 x y y' A :
-  x <> y -> y <> y' -> x <> y' -> 
-  Alpha3 (tmlam x A (tmlam y A (tmapp (tmvar x) (tmvar y)))) (tmlam y A (tmlam y' A (tmapp (tmvar y) (tmvar y')))).
-Proof.
-  intros.
-  econstructor; auto.
-  simpl.
-  destr_eqb_eq x y; try contradiction.
-  apply fresh3_sound_complete.
-  simpl.
-  rewrite String.eqb_refl.
-  destr_eqb_eq y x; try contradiction.
-  rewrite String.eqb_refl.
-  destr_eqb_eq y y'; try contradiction.
-  destr_eqb_eq x y; try contradiction.
-  econstructor; auto.
-  apply fresh3_sound_complete.
-  simpl.
-  remember (fresh3 x y _ _) as fr1.
-  remember (fresh3 y y' _ _) as fr2.
-  assert (y =? fr1 = false) by admit.
-  rewrite H5.
-  assert (y' =? fr1 = false) by admit; rewrite H6.
-  repeat rewrite String.eqb_refl.
-  repeat constructor; auto.
-Admitted.
-
-
-Lemma alpha2_exampl x y y' A :
-  x <> y -> y <> y' -> x <> y' -> 
-  Alpha2 (tmlam x A (tmlam y A (tmapp (tmvar x) (tmvar y)))) (tmlam y A (tmlam y' A (tmapp (tmvar y) (tmvar y')))).
-Proof.
-  intros Hxy Hyy' Hxy'.
-  apply alpha2_lam.
-  simpl.
-  destr_eqb_eq x y; try contradiction.
-  destr_eqb_eq y y'; try contradiction.
-  apply alpha2_lam.
-  simpl.
-  apply alpha2_app.
-  repeat rewrite String.eqb_refl.
-  simpl.
-  rewrite String.eqb_refl.
-  destr_eqb_eq y y'; try contradiction.
-  destr_eqb_eq y' y; try contradiction.
-Abort. (* doesnt work *)
-
-
 (* Showcasing shadowing behaviour is right *)
 Lemma alpha_counterexample x y z A :
   x <> y -> x <> z -> y <> z -> 
-  (Alpha [] (tmlam x A (tmlam y A (tmapp (tmvar x) (tmvar y)))) 
-    (tmlam z A (tmlam z A (tmapp (tmvar z) (tmvar z)))) -> False).
+  (Alpha [] (@tmlam Lam x A (@tmlam Lam y A (@tmapp App (tmvar x) (tmvar y)))) 
+    (@tmlam Lam z A (@tmlam Lam z A (@tmapp App (tmvar z) (tmvar z)))) -> False).
 Proof.
   intros Hxy Hxz Hyz Halpha.
   inversion Halpha; subst.
   inversion H1; subst.
   inversion H2; subst.
-  inversion H5; subst.
   inversion H4; subst.
-  - contradiction Hxy. reflexivity.
-  - contradiction H10. reflexivity.
-Qed.
-
-(* Showcasing shadowing behaviour is right *)
-Lemma alpha3_counterexample x y z A :
-  x <> y -> x <> z -> y <> z -> 
-  (Alpha3 (tmlam x A (tmlam y A (tmapp (tmvar x) (tmvar y)))) 
-    (tmlam z A (tmlam z A (tmapp (tmvar z) (tmvar z)))) -> False).
-Proof.
-  intros Hxy Hxz Hyz Halpha.
-  inversion Halpha; subst.
-  simpl in H5.
-  repeat rewrite String.eqb_refl in H5.
-  assert (x =? y = false) by admit.
-  rewrite H in H5.
   inversion H5; subst.
-  simpl in H8.
-  assert (y =? fr = false) by admit.
-  rewrite H0 in H8.
-  repeat rewrite String.eqb_refl in H8.
-  inversion H8; subst.
-  inversion H7; subst.
-  (* Contradiction in H3: fr0 is not fresh over tmapp (tmvar fr0) (tmvar y))*)
-Admitted.
+  - contradiction Hxy. subst. reflexivity. 
+  - contradiction.
+Qed.
 
 Lemma alpha_var_id {x y z}:
   AlphaVar [] x y -> AlphaVar [(z, z)] x y.
@@ -708,6 +489,7 @@ Proof.
   - apply alpha_app.
     + exact (IHHalpha1 ren' lrs).
     + exact (IHHalpha2 ren' lrs).
+  - constructor.
 Qed.
 
 (* In particular we can now swap identity renamings *)
@@ -952,6 +734,7 @@ Proof.
   - apply alpha_app.
     + apply IHHalpha1; auto.
     + apply IHHalpha2; auto.
+  - constructor.
 Qed.
 
 Lemma alpha_extend_ids_right s t ren idCtx:
@@ -1052,8 +835,8 @@ Alpha [] (tmlam x A (tmlam x A x)) (tmlam x A (tmlam y A y))
 
 We do not yet use this. Just checking if the alpha machinery is powerful enough
 *)
-Lemma freshVarAlpha x s t A :
-  Alpha [] s t -> Alpha [] (tmlam x A s) (tmlam x A t).
+Lemma freshVarAlpha B x s t A :
+  Alpha [] s t -> Alpha [] (@tmlam B x A s) (@tmlam B x A t).
 Proof. 
   intros Halpha.
   apply alpha_lam.
@@ -1097,6 +880,7 @@ Proof.
     apply alpha_app;
     [apply IHs1 | apply IHs2]; 
     now apply not_in_app in Hfresh as [Hfresh1 Hfresh2].
+  - constructor.
 Qed.
 
 (* WHY DO WE HAVE THIS? WHY NOT FTV?*)
